function method

examples/iterators/ElimDupNoIts.dfy
@@ -1,36 +1,24 @@
 include "../../src/linear/layer1/List.dfy"
 include "../../src/linear/layer2/LinkedList.dfy"
 include "../../src/linear/layer2/ArrayList.dfy"
-include "../../src/Order.dfy"
+include "../../src/UtilsAux.dfy"
 
-predicate Sorted<A>(xs: seq<A>,le:(A,A)->bool)
-requires IsTotalOrder(le)
-{
-  forall i, j :: 0 <= i <= j < |xs| ==> le(xs[i],xs[j])
-}
-
-predicate StrictSorted<A>(xs: seq<A>,le:(A,A)->bool)
-requires IsTotalOrder(le)
-{
-  forall i, j :: 0 <= i < j < |xs| ==> (le(xs[i],xs[j]) && !le(xs[j],xs[i])) 
-}
-
-method ElimDup<A>(l:List<A>,le:(A,A)->bool)
+method ElimDup(l:LinkedList<int>)
 //method {:verify true} elimDupA(l:ArrayList<int>) //NO CHANGES
  modifies l, l.Repr()
  requires allocated(l.Repr())
  ensures fresh(l.Repr()-old(l.Repr()))
  ensures allocated(l.Repr())
- requires IsTotalOrder(le)
 
- requires l.Valid() && Sorted(l.Model(),le)
+ requires l.Valid() && Sorted(l.Model())
  ensures l.Valid()
 
  ensures (set x | x in old(l.Model())) == (set x | x in l.Model())
- ensures StrictSorted(l.Model(),le)
+ ensures StrictSorted(l.Model())
 
  ensures l.Iterators() >= old(l.Iterators())
 {
+  
   var it2 := l.First();
   var it1 := it2.Copy();
   var b := it1.HasPeek();
@@ -52,26 +40,23 @@ method ElimDup<A>(l:List<A>,le:(A,A)->bool)
 
       invariant l.Valid()
       invariant it2 in l.Iterators() && it1 in l.Iterators()
-      invariant it1.Parent() == l && it2.Parent() == l
+      invariant it1.Parent() == l && it2.Parent()==l
       invariant it1.Valid() && it2.Valid()
-      invariant it1.Index() >= 0
       invariant it2.Index() == it1.Index()+1
       invariant it2.HasPeek?() ==> it1.HasPeek?() && l.Model()[it1.Index()+1] == l.Model()[it2.Index()]
 
       invariant (set x | x in old(l.Model())) == (set x | x in l.Model())
-      invariant Sorted(l.Model(),le) && StrictSorted(l.Model()[..it2.Index()],le)
+      invariant Sorted(l.Model()) && StrictSorted(l.Model()[..it2.Index()])
       invariant b == it2.HasPeek?()
 
       invariant l.Iterators() >= old(l.Iterators())
     {
      var it1Peek := it1.Peek();
      var it2Peek := it2.Peek();
-     if (le(it1Peek,it2Peek) && le(it2Peek,it1Peek)) 
-     {
-        assert it1Peek == it2Peek;
-        ghost var oit2 := it2.Index();
+     if (it1Peek == it2Peek) {
         it2 := l.Erase(it2);
-      } else {
+     } 
+     else {
         it2.Next();
         it1.Next();
       }
